
# Approach 1:

A common and efficient approach to solve this problem is by using the **mathematical formula for the sum of the first nnn natural numbers**.

#### Mathematical Approach:

1. **Sum of First nnn Natural Numbers**: The sum of the first nnn natural numbers can be calculated using the formula:
    
    Sum=n×(n+1)2\text{Sum} = \frac{n \times (n + 1)}{2}Sum=2n×(n+1)​
    
    Where nnn is the length of the input array.
    
2. **Calculate the Expected Sum**: Calculate the expected sum of numbers from `0` to `n` using the formula above.
    
3. **Calculate the Actual Sum**: Sum the elements present in the given array.
    
4. **Find the Missing Number**: The missing number can be found by subtracting the actual sum from the expected sum:
    
    Missing Number=Expected Sum−Actual Sum\text{Missing Number} = \text{Expected Sum} - \text{Actual Sum}Missing Number=Expected Sum−Actual Sum
### Complexity Analysis

- **Time Complexity**: O(n)O(n)O(n) - The time complexity is linear because we iterate through the array once to compute the actual sum.
- **Space Complexity**: O(1)O(1)O(1) - The space complexity is constant because we are only using a fixed amount of extra space (for the sums).


```python
class Solution:
    def missingNumber(self, nums: List[int]) -> int:
        n = len(nums)
        expected_sum = n * (n + 1) // 2  # Using integer division
        actual_sum = sum(nums)
        return expected_sum - actual_sum


```

### Dry Run Example

Let’s dry run this algorithm with the input array `nums = [3, 0, 1]`.

1. **Input**:
    
    plaintext
    
    Copy code
    
    `nums = [3, 0, 1] n = 3 (length of the array)`
    
2. **Calculate the Expected Sum**:
    
    Expected Sum=3×(3+1)2=3×42=6\text{Expected Sum} = \frac{3 \times (3 + 1)}{2} = \frac{3 \times 4}{2} = 6Expected Sum=23×(3+1)​=23×4​=6
3. **Calculate the Actual Sum**:
    
    Actual Sum=3+0+1=4\text{Actual Sum} = 3 + 0 + 1 = 4Actual Sum=3+0+1=4
4. **Find the Missing Number**:
    
    Missing Number=Expected Sum−Actual Sum=6−4=2\text{Missing Number} = \text{Expected Sum} - \text{Actual Sum} = 6 - 4 = 2Missing Number=Expected Sum−Actual Sum=6−4=2